4-25

nmap_assign.thy
@@ -1,133 +1,38 @@
-section \<open> Alphabetised Relations \<close>
-
 theory nmap_assign
 imports
   nmap_expr
-
 begin
 
-text \<open> An alphabetised relation is simply a predicate whose state-space is a product type. In this
-  theory we construct the core operators of the relational calculus, and prove a libary of 
-  associated theorems, based on Chapters 2 and 5 of the UTP book~\cite{Hoare&98}. \<close>
-  
-subsection \<open> Relational Alphabets \<close>
-  
-text \<open> We set up convenient syntax to refer to the input and output parts of the alphabet, as is
-  common in UTP. Since we are in a product space, these are simply the lenses @{term "fst\<^sub>L"} and
-  @{term "snd\<^sub>L"}. \<close>
-  
-definition in\<alpha> :: "('\<alpha> \<Longrightarrow> '\<alpha> \<times> '\<beta>)" where
-[lens_defs]: "in\<alpha> = fst\<^sub>L"
+(***
+typedef '\<alpha> proc  = "UNIV :: (bool, '\<alpha> \<times> '\<alpha>) uexpr set" ..
+***)
+type_synonym '\<alpha> proc        = " (bool, '\<alpha> \<times> '\<alpha>) uexpr"
+type_synonym ('a, '\<alpha>) aproc = " ('a, '\<alpha> \<times> '\<alpha>) uexpr"
+type_synonym ('\<alpha>, '\<beta>) urel  = " (bool, '\<alpha> \<times> '\<beta>) uexpr"
 
-definition out\<alpha> :: "('\<beta> \<Longrightarrow> '\<alpha> \<times> '\<beta>)" where
-[lens_defs]: "out\<alpha> = snd\<^sub>L"
+subsection \<open> assignment statement  \<close>
 
-lemma in\<alpha>_uvar [simp]: "vwb_lens in\<alpha>"
-  by (unfold_locales, auto simp add: in\<alpha>_def)
-
-lemma out\<alpha>_uvar [simp]: "vwb_lens out\<alpha>"
-  by (unfold_locales, auto simp add: out\<alpha>_def)
-
-lemma var_in_alpha [simp]: "x ;\<^sub>L in\<alpha> = ivar x"
-  by (simp add: fst_lens_def in\<alpha>_def in_var_def)
-
-lemma var_out_alpha [simp]: "x ;\<^sub>L out\<alpha> = ovar x"
-  by (simp add: out\<alpha>_def out_var_def snd_lens_def)
-
-lemma out_alpha_in_indep [simp]:
-  "out\<alpha> \<bowtie> in_var x" "in_var x \<bowtie> out\<alpha>"
-  by (simp_all add: in_var_def out\<alpha>_def lens_indep_def fst_lens_def snd_lens_def lens_comp_def)
-
-lemma in_alpha_out_indep [simp]:
-  "in\<alpha> \<bowtie> out_var x" "out_var x \<bowtie> in\<alpha>"
-  by (simp_all add: in_var_def in\<alpha>_def lens_indep_def fst_lens_def lens_comp_def)
-
-text \<open> The following two functions lift a predicate substitution to a relational one. \<close>
- 
-abbreviation usubst_rel_lift :: "'\<alpha> usubst \<Rightarrow> ('\<alpha> \<times> '\<beta>) usubst" ("\<lceil>_\<rceil>\<^sub>s") where
-"\<lceil>\<sigma>\<rceil>\<^sub>s \<equiv> \<sigma> \<oplus>\<^sub>s in\<alpha>"
-
-abbreviation usubst_rel_drop :: "('\<alpha> \<times> '\<alpha>) usubst \<Rightarrow> '\<alpha> usubst" ("\<lfloor>_\<rfloor>\<^sub>s") where
-"\<lfloor>\<sigma>\<rfloor>\<^sub>s \<equiv> \<sigma> \<restriction>\<^sub>s in\<alpha>"
-
-text \<open> The alphabet of a relation then consists wholly of the input and output portions. \<close>
-
-lemma alpha_in_out:
-  "\<Sigma> \<approx>\<^sub>L in\<alpha> +\<^sub>L out\<alpha>"
-  by (simp add: fst_snd_id_lens in\<alpha>_def lens_equiv_refl out\<alpha>_def)
-
-subsection \<open> Relational Types and Operators \<close>
-
-text \<open> We create type synonyms for conditions (which are simply predicates) -- i.e. relations
-  without dashed variables --, alphabetised relations where the input and output alphabet can
-  be different, and finally homogeneous relations. \<close>
-type_synonym '\<alpha> hrel        = " (bool, '\<alpha> \<times> '\<alpha>) uexpr"
-
-text \<open> We set up some overloaded constants for sequential composition and the identity in case
-  we want to overload their definitions later. \<close>
-  
 consts
-  useq     :: "'a \<Rightarrow> 'b \<Rightarrow> 'c" (infixr ";;" 61)
   uassigns :: "'a usubst \<Rightarrow> 'b" ("\<langle>_\<rangle>\<^sub>a")
   uskip    :: "'a" ("II")
-  
 
-
-text \<open> Assignment is defined using substitutions, where latter defines what each variable should
-  map to. The definition of the operator identifies the after state binding, $b'$, with the 
-  substitution function applied to the before state binding $b$. \<close>
-  
-lift_definition assigns_r :: "'\<alpha> usubst \<Rightarrow> '\<alpha> hrel "
+lift_definition assigns_r :: "'\<alpha> usubst \<Rightarrow> '\<alpha> proc "
   is "\<lambda> \<sigma> (b, b'). b' = \<sigma>(b)" .
 
 adhoc_overloading
   uassigns assigns_r
     
-text \<open> Relational identity, or skip, is then simply an assignment with the identity substitution:
-  it simply identifies all variables. \<close>
-    
-definition skip_r :: " '\<alpha> hrel " where"skip_r = assigns_r id"
+definition skip_r :: " '\<alpha> proc " where "skip_r = assigns_r id"
 
 adhoc_overloading
   uskip skip_r
- 
-text \<open> A singleton assignment simply applies a singleton substitution function, and similarly
-  for a double assignment. \<close>
-
-abbreviation assign_r :: "('t \<Longrightarrow> '\<alpha>) \<Rightarrow> ('t, '\<alpha>) uexpr \<Rightarrow> '\<alpha> hrel "
-where "assign_r x v \<equiv> \<langle>[x \<mapsto>\<^sub>s v]\<rangle>\<^sub>a"
-
-abbreviation assign_2_r ::
-  "('t1 \<Longrightarrow> '\<alpha>) \<Rightarrow> ('t2 \<Longrightarrow> '\<alpha>) \<Rightarrow> ('t1, '\<alpha>) uexpr \<Rightarrow> ('t2, '\<alpha>) uexpr \<Rightarrow> '\<alpha> hrel "
-where "assign_2_r x y u v \<equiv> assigns_r [x \<mapsto>\<^sub>s u, y \<mapsto>\<^sub>s v]"
-
-text \<open> We also define the alphabetised skip operator that identifies all input and output variables
-  in the given alphabet lens. All other variables are unrestricted. We also set up syntax for it. \<close>
-  
-definition skip_ra :: "('\<beta>, '\<alpha>) lens \<Rightarrow>  '\<alpha> hrel " where "skip_ra v = ($v\<acute> =\<^sub>u $v)"
-
-text \<open> Similarly, we define the alphabetised assignment operator. \<close>
-
-definition assigns_ra :: "'\<alpha> usubst \<Rightarrow> ('\<beta>, '\<alpha>) lens \<Rightarrow> '\<alpha> hrel " ("\<langle>_\<rangle>\<^bsub>_\<^esub>") where
-"\<langle>\<sigma>\<rangle>\<^bsub>a\<^esub> = (\<lceil>\<sigma>\<rceil>\<^sub>s \<dagger> skip_ra a)"
-
-
-
-
-
-
-
-
-
-subsection \<open> Syntax Translations \<close>
     
 syntax
   \<comment> \<open> Single and multiple assignement \<close>
-  "_assignment"     :: "svids \<Rightarrow> uexprs \<Rightarrow> '\<alpha> hrel"  ("'(_') := '(_')")  
-  "_assignment"     :: "svids \<Rightarrow> uexprs \<Rightarrow> '\<alpha> hrel"  (infixr ":=" 62)
+  "_assignment"     :: "svids \<Rightarrow> uexprs \<Rightarrow> '\<alpha> proc"  ("'(_') := '(_')")  
+  "_assignment"     :: "svids \<Rightarrow> uexprs \<Rightarrow> '\<alpha> proc"  (infixr ":=" 62)
   \<comment> \<open> Substitution constructor \<close>
   "_mk_usubst"      :: "svids \<Rightarrow> uexprs \<Rightarrow> '\<alpha> usubst"
-
 
 translations
   "_mk_usubst \<sigma> (_svid_unit x) v" \<rightleftharpoons> "\<sigma>(&x \<mapsto>\<^sub>s v)"
@@ -138,58 +43,73 @@ translations
   "x,y := u,v" <= "CONST uassigns (CONST subst_upd (CONST subst_upd (CONST id) (CONST svar x) u) (CONST svar y) v)"
 
 (***    test begin    ***)
-lemma assign_vacuous_skip:
+lemma assign_skip:
   assumes "vwb_lens x"
   shows "(x := &x) = II"
   by (metis assms pr_var_def skip_r_def usubst_upd_pr_var_id)
   
-lemma assign_simultaneous:
+lemma assign_simul1:
   assumes "vwb_lens y" "x \<bowtie> y"
-  shows "(x,y) := (e, &y) = (x := e)"
-  by (simp add: assms usubst_upd_comm usubst_upd_var_id)
+  shows "(x,y) := (1+1, &y) = (x := 2)"
+  by (metis assms(1) assms(2) one_add_one pr_var_def usubst_upd_comm usubst_upd_pr_var_id)
 
-lemma assigns_idem: "mwb_lens x \<Longrightarrow> (x,x) := (u,v) = (x := v)"
-  by (simp add: usubst)
-
-alphabet state =
-  a :: int
-  b :: int 
-  c :: int
-
-text \<open> Prove a simple relational equality \<close>
-  
-theorem "(a,b) := (2, &b) = (a := 2)"
-  by (simp add:  usubst_upd_comm usubst_upd_var_id)
-
-theorem "(a,b) := (2, &a+1) = (a,b) := (2,&a+1)"
-  by simp
-
-theorem "(a,b,c) := (2, &b, 4) = (a,c) := (2,4)"
-  by (metis b_vwb_lens pr_var_def state_indeps(1) usubst_upd_comm usubst_upd_pr_var_id)
-
-theorem "(b := 3) = (b,a) := (3 ,&a)"
-  by (simp add:  usubst_upd_comm usubst_upd_var_id)
-
-lemma "a \<bowtie> b"
-  by simp
-
-lemma assign_simueweltaus:
-  assumes "vwb_lens a" "a \<bowtie> b"
-  shows "(a,b) := (3, &b) = (a := 3)"
-  by (simp add: assms usubst_upd_comm usubst_upd_var_id)
-(***   test end   ***)
+lemma assigns_simul2: "vwb_lens x \<Longrightarrow> (x,x) := (u,v) = (x := v)"
+  by (simp add: subst_upd_pr_var usubst_upd_idem)
+(***    test end    ***)
 
 
-class nchoice = 
-  fixes nchoice :: "'a hrel \<Rightarrow> 'a hrel \<Rightarrow> 'a hrel" (infixl "\<sqinter>" 70)
+
+
+
+
+
+subsection \<open> serial statement  \<close>
+locale serial = 
+  fixes serial :: "'\<alpha> proc \<Rightarrow> '\<alpha> proc \<Rightarrow> '\<alpha> proc" (infixl ";;" 60)
+  assumes serial_assoc : "(X ;; Y) ;; Z = X ;; (Y ;; Z)"
+      and serial_skip_left : "II ;;X = X"
+      and serial_skip_right : "X ;; II = X"
+
+lemma  (in serial) assign_test1:
+  assumes "vwb_lens x"
+  shows "(x:=1  ;; II) = x := 1"
+  using serial_skip_right by auto
+
+
+lemma  (in serial) assign_test2:
+  assumes "vwb_lens y"  "vwb_lens x" "x \<bowtie> y"
+  shows "(x:=1  ;; y:=2) = (x,y) := (1,2)"
+ (***     can not proof  ***)
+
+
+(***
+consts
+  useq     :: "'a \<Rightarrow> 'b \<Rightarrow> 'c" (infixr ";;" 61)
+
+lift_definition seqr:: "'\<alpha> proc \<Rightarrow> '\<alpha> proc \<Rightarrow> '\<alpha> proc"
+is "\<lambda> P Q b. b \<in> ({p. P p} O {q. Q q})" .
+
+adhoc_overloading
+  useq seqr
+***)
+
+
+
+
+subsection \<open> nchoice statement  \<close>
+
+locale nchoice = 
+  fixes nchoice :: "'\<alpha> proc \<Rightarrow> '\<alpha> proc \<Rightarrow> '\<alpha> proc" (infixl "\<sqinter>" 70)
   assumes nch_assoc [algebra_simps, field_simps]: "(x \<sqinter> y) \<sqinter> z = x \<sqinter> (y \<sqinter> z)"
       and nch_commute [algebra_simps, field_simps]: "x \<sqinter> y = y \<sqinter> x"
       and nch_idemp [algebra_simps, field_simps]: "(x \<sqinter> x) = x" 
       and nch_skip_left: " II \<sqinter> x = x"
       and nch_skip_right: "x \<sqinter>  II = x"
 
-lemma " (x:=3)  \<sqinter> (y:=4) =  (y:=4)  \<sqinter>  (x:=3)  "
+lemma (in nchoice) "(x:=3)  \<sqinter> (y:=4) =  (y:=4)  \<sqinter>  (x:=3)"
   by (simp add: nch_commute)
+
+
 
 (***
 lemma " (a:=3)  \<sqinter> (b:=4) =  (b:=4)  \<sqinter>  (a:=3)  "
@@ -197,13 +117,20 @@ lemma " (a:=3)  \<sqinter> (b:=4) =  (b:=4)  \<sqinter>  (a:=3)  "
 ***)
 
 
-definition ifprog :: " 'a hrel  \<Rightarrow> bool \<Rightarrow> 'a hrel \<Rightarrow> 'a hrel"  ("(_ \<triangleleft> _  \<triangleright>\<^sub>\<p>/ _)" [52,0,53] 52)
-  where "x  \<triangleleft> P  \<triangleright>\<^sub>\<p> y \<equiv> (THE z::'a hrel. (P = True \<longrightarrow> z = x) \<and> (P = False \<longrightarrow> z = y))"
+
+subsection \<open> if-than-else statement  \<close>
+
+definition ifprog :: " 'a  \<Rightarrow> bool \<Rightarrow> 'a  \<Rightarrow> 'a "  ("(_ \<triangleleft> _  \<triangleright>\<^sub>\<p>/ _)" [52,0,53] 52)
+  where "x  \<triangleleft> P  \<triangleright>\<^sub>\<p> y \<equiv> (THE z::'a . (P = True \<longrightarrow> z = x) \<and> (P = False \<longrightarrow> z = y))"
 
 theorem ifprog_idemp : "x \<triangleleft> boole \<triangleright>\<^sub>\<p> x = x"
   by (simp add: ifprog_def)
 
-theorem  "(a:=5) \<triangleleft> True \<triangleright>\<^sub>\<p> (b:=6) = (a:=5)"
-  by (simp add: ifprog_def)
+
+
+
+
+
+
 
 end
