nmap_var.thy
@@ -1,14 +1,11 @@
-theory nmap_var
+theory nmap_var 
 imports "./Optics/Lenses"   "HOL-Library.Adhoc_Overloading"
 begin
 
-definition in_var :: "('a \<Longrightarrow> '\<alpha>) \<Rightarrow> ('a \<Longrightarrow> '\<alpha> \<times> '\<beta>)" where
-[lens_defs]: "in_var x = x ;\<^sub>L fst\<^sub>L"
+definition var :: "('a \<Longrightarrow> '\<alpha>) \<Rightarrow> ('a \<Longrightarrow> '\<alpha>)" where
+[lens_defs]: "var x = x"    
 
-definition out_var :: "('a \<Longrightarrow> '\<beta>) \<Rightarrow> ('a \<Longrightarrow> '\<alpha> \<times> '\<beta>)" where
-[lens_defs]: "out_var x = x ;\<^sub>L snd\<^sub>L"
-
-abbreviation (input) univ_alpha :: "('\<alpha> \<Longrightarrow> '\<alpha>)" ("\<Sigma>") where
+definition univ_alpha :: "('\<alpha> \<Longrightarrow> '\<alpha>)" ("\<Sigma>") where
 "univ_alpha \<equiv> 1\<^sub>L"
 
 definition pr_var :: "('a \<Longrightarrow> '\<beta>) \<Rightarrow> ('a \<Longrightarrow> '\<beta>)" where
@@ -33,8 +30,6 @@ consts
 syntax 
 \<comment> \<open> Decorations \<close>
   "_spvar"       :: "svid \<Rightarrow> svar" ("&_" [990] 990)
-  "_sinvar"      :: "svid \<Rightarrow> svar" ("$_" [990] 990)
-  "_soutvar"     :: "svid \<Rightarrow> svar" ("$_\<acute>" [990] 990)
  \<comment> \<open> Variable sets \<close>
   "_salphaid"    :: "svid \<Rightarrow> salpha" ("_" [990] 990)
   "_salphavar"   :: "svar \<Rightarrow> salpha" ("_" [990] 990)
@@ -58,15 +53,9 @@ translations
   "_svid_dot x y" \<rightharpoonup> "y ;\<^sub>L x"
 \<comment> \<open> Decorations \<close>
   "_spvar \<Sigma>"  \<leftharpoondown>  "CONST svar CONST id_lens"
-  "_sinvar \<Sigma>"  \<leftharpoondown> "CONST ivar 1\<^sub>L"
-  "_soutvar \<Sigma>" \<leftharpoondown> "CONST ovar 1\<^sub>L"
   "_spvar (_svid_dot x y)" \<leftharpoondown> "CONST svar (CONST lens_comp y x)"
-  "_sinvar (_svid_dot x y)" \<leftharpoondown> "CONST ivar (CONST lens_comp y x)"
-  "_soutvar (_svid_dot x y)" \<leftharpoondown> "CONST ovar (CONST lens_comp y x)"
   "_svid_dot (_svid_dot x y) z" \<leftharpoondown> "_svid_dot (CONST lens_comp y x) z"
   "_spvar x" \<rightleftharpoons> "CONST svar x"
-  "_sinvar x" \<rightleftharpoons> "CONST ivar x"
-  "_soutvar x" \<rightleftharpoons> "CONST ovar x"
 \<comment> \<open> Alphabets \<close>
   "_salphaparen a" \<rightharpoonup> "a"
   "_salphaid x" \<rightharpoonup> "x"
@@ -87,8 +76,7 @@ translations
 adhoc_overloading
   svar pr_var and ivar in_var and ovar out_var
 
-syntax
-  "_uvar_ty"  :: "type \<Rightarrow> type \<Rightarrow> type"
+
 
 
 
@@ -104,77 +92,25 @@ declare comp_vwb_lens [simp]
 declare lens_indep_left_ext [simp]
 declare lens_indep_right_ext [simp]
 
-text \<open> We can now easily show that our UTP variable construction are various classes of 
-  well-behaved lens .\<close>
+text \<open> We can now easily show that our UTP variable construction are various classes of  well-behaved lens .\<close>
 
-lemma in_var_weak_lens [simp]:
-  "weak_lens x \<Longrightarrow> weak_lens (in_var x)"
-  by (simp add: comp_weak_lens in_var_def)
+lemma var_uvar [simp]:
+  "vwb_lens x \<Longrightarrow> vwb_lens (var x)"
+  by (simp add: var_def)
 
-lemma in_var_semi_uvar [simp]:
-  "mwb_lens x \<Longrightarrow> mwb_lens (in_var x)"
-  by (simp add: comp_mwb_lens in_var_def)
-
-lemma pr_var_weak_lens [simp]:
-  "weak_lens x \<Longrightarrow> weak_lens (pr_var x)"
-  by (simp add: pr_var_def)
-
-lemma pr_var_mwb_lens [simp]:
-  "mwb_lens x \<Longrightarrow> mwb_lens (pr_var x)"
-  by (simp add: pr_var_def)
-    
 lemma pr_var_vwb_lens [simp]: 
   "vwb_lens x \<Longrightarrow> vwb_lens (pr_var x)"
   by (simp add: pr_var_def)
     
-lemma in_var_uvar [simp]:
-  "vwb_lens x \<Longrightarrow> vwb_lens (in_var x)"
-  by (simp add: in_var_def)
-
-lemma out_var_weak_lens [simp]:
-  "weak_lens x \<Longrightarrow> weak_lens (out_var x)"
-  by (simp add: comp_weak_lens out_var_def)
-
-lemma out_var_semi_uvar [simp]:
-  "mwb_lens x \<Longrightarrow> mwb_lens (out_var x)"
-  by (simp add: comp_mwb_lens out_var_def)
-
-lemma out_var_uvar [simp]:
-  "vwb_lens x \<Longrightarrow> vwb_lens (out_var x)"
-  by (simp add: out_var_def)
-    
-text \<open> Moreover, we can show that input and output variables are independent, since they refer
-  to different sections of the alphabet. \<close>
-    
-lemma in_out_indep [simp]:
-  "in_var x \<bowtie> out_var y"
-  by (simp add: lens_indep_def in_var_def out_var_def fst_lens_def snd_lens_def lens_comp_def)
-
-lemma out_in_indep [simp]:
-  "out_var x \<bowtie> in_var y"
-  by (simp add: lens_indep_def in_var_def out_var_def fst_lens_def snd_lens_def lens_comp_def)
-
 lemma in_var_indep [simp]:
-  "x \<bowtie> y \<Longrightarrow> in_var x \<bowtie> in_var y"
-  by (simp add: in_var_def out_var_def)
-
-lemma out_var_indep [simp]:
-  "x \<bowtie> y \<Longrightarrow> out_var x \<bowtie> out_var y"
-  by (simp add: out_var_def)
+  "x \<bowtie> y \<Longrightarrow> var x \<bowtie> var y"
+  by (simp add: var_def)
 
 lemma pr_var_indeps [simp]: 
   "x \<bowtie> y \<Longrightarrow> pr_var x \<bowtie> y"
   "x \<bowtie> y \<Longrightarrow> x \<bowtie> pr_var y"
   by (simp_all add: pr_var_def)
     
-lemma prod_lens_indep_in_var [simp]:
-  "a \<bowtie> x \<Longrightarrow> a \<times>\<^sub>L b \<bowtie> in_var x"
-  by (metis in_var_def in_var_indep out_in_indep out_var_def plus_pres_lens_indep prod_as_plus)
-
-lemma prod_lens_indep_out_var [simp]:
-  "b \<bowtie> x \<Longrightarrow> a \<times>\<^sub>L b \<bowtie> out_var x"
-  by (metis in_out_indep in_var_def out_var_def out_var_indep plus_pres_lens_indep prod_as_plus)
-
 lemma in_var_pr_var [simp]:
   "in_var (pr_var x) = in_var x"
   by (simp add: pr_var_def)
@@ -195,41 +131,12 @@ lemma pr_var_lens_comp_1 [simp]:
   "pr_var x ;\<^sub>L y = pr_var (x ;\<^sub>L y)"
   by (simp add: pr_var_def)
     
-lemma in_var_plus [simp]: "in_var (x +\<^sub>L y) = in_var x +\<^sub>L in_var y"
-  by (simp add: in_var_def plus_lens_distr)
+lemma var_plus [simp]: "var (x +\<^sub>L y) = var x +\<^sub>L var y"
+  by (simp add: var_def plus_lens_distr)
 
-lemma out_var_plus [simp]: "out_var (x +\<^sub>L y) = out_var x +\<^sub>L out_var y"
-  by (simp add: out_var_def plus_lens_distr)
-  
-text \<open> Similar properties follow for sublens \<close>
-  
-lemma in_var_sublens [simp]:
-  "y \<subseteq>\<^sub>L x \<Longrightarrow> in_var y \<subseteq>\<^sub>L in_var x"
-  by (metis (no_types, hide_lams) in_var_def lens_comp_assoc sublens_def)
-     
-lemma out_var_sublens [simp]:
-  "y \<subseteq>\<^sub>L x \<Longrightarrow> out_var y \<subseteq>\<^sub>L out_var x"
-  by (metis (no_types, hide_lams) out_var_def lens_comp_assoc sublens_def)
 
-lemma pr_var_sublens [simp]:
-  "y \<subseteq>\<^sub>L x \<Longrightarrow> pr_var y \<subseteq>\<^sub>L pr_var x"
-  by (simp add: pr_var_def)
 
-subsection \<open> Lens simplifications \<close>
-    
-text \<open> We also define some lookup abstraction simplifications. \<close>
 
-lemma var_lookup_in [simp]: "lens_get (in_var x) (A, A') = lens_get x A"
-  by (simp add: in_var_def fst_lens_def lens_comp_def)
-
-lemma var_lookup_out [simp]: "lens_get (out_var x) (A, A') = lens_get x A'"
-  by (simp add: out_var_def snd_lens_def lens_comp_def)
-
-lemma var_update_in [simp]: "lens_put (in_var x) (A, A') v = (lens_put x A v, A')"
-  by (simp add: in_var_def fst_lens_def lens_comp_def)
-
-lemma var_update_out [simp]: "lens_put (out_var x) (A, A') v = (A, lens_put x A' v)"
-  by (simp add: out_var_def snd_lens_def lens_comp_def)
 
 
 
