nmap_expr.thy
@@ -6,13 +6,13 @@ subsection \<open> Expression type \<close>
 
 no_notation BNF_Def.convol ("\<langle>(_,/ _)\<rangle>")
 
-typedef ('t, '\<alpha>) uexpr = "UNIV :: ('\<alpha> \<Rightarrow> 't) set" ..
+text \<open>the following make a new type called uexpr.then using lifting makes uexpr support var lit uop and bot\<close>
 
+typedef ('t, '\<alpha>) uexpr = "UNIV :: ('\<alpha> \<Rightarrow> 't) set" ..
 
 notation Rep_uexpr ("\<lbrakk>_\<rbrakk>\<^sub>e")
 
-lemma uexpr_eq_iff:
-  "e = f \<longleftrightarrow> (\<forall> b. \<lbrakk>e\<rbrakk>\<^sub>e b = \<lbrakk>f\<rbrakk>\<^sub>e b)"
+lemma uexpr_eq_iff: "e = f \<longleftrightarrow> (\<forall> b. \<lbrakk>e\<rbrakk>\<^sub>e b = \<lbrakk>f\<rbrakk>\<^sub>e b)"
   using Rep_uexpr_inject[of e f, THEN sym] by (auto)
 
 setup_lifting type_definition_uexpr
@@ -21,7 +21,7 @@ named_theorems uexpr_defs and ueval and lit_simps and lit_norm
 subsection \<open> Core expression constructs using lift_definition  \<close>
 
 lift_definition var :: "('t \<Longrightarrow> '\<alpha>) \<Rightarrow> ('t, '\<alpha>) uexpr" is lens_get .
-
+                                                             
 lift_definition lit :: "'t \<Rightarrow> ('t, '\<alpha>) uexpr" ("\<guillemotleft>_\<guillemotright>") is "\<lambda> v b. v" .
 
 lift_definition uop :: "('a \<Rightarrow> 'b) \<Rightarrow> ('a, '\<alpha>) uexpr \<Rightarrow> ('b, '\<alpha>) uexpr"
@@ -31,25 +31,13 @@ lift_definition bop ::
   "('a \<Rightarrow> 'b \<Rightarrow> 'c) \<Rightarrow> ('a, '\<alpha>) uexpr \<Rightarrow> ('b, '\<alpha>) uexpr \<Rightarrow> ('c, '\<alpha>) uexpr"
   is "\<lambda> f u v b. f (u b) (v b)" .
 
-lift_definition trop ::
-  "('a \<Rightarrow> 'b \<Rightarrow> 'c \<Rightarrow> 'd) \<Rightarrow> ('a, '\<alpha>) uexpr \<Rightarrow> ('b, '\<alpha>) uexpr \<Rightarrow> ('c, '\<alpha>) uexpr \<Rightarrow> ('d, '\<alpha>) uexpr"
-  is "\<lambda> f u v w b. f (u b) (v b) (w b)" .
-
-lift_definition ulambda :: "('a \<Rightarrow> ('b, '\<alpha>) uexpr) \<Rightarrow> ('a \<Rightarrow> 'b, '\<alpha>) uexpr"
-is "\<lambda> f A x. f x A" .
 
 
 
-definition uIf :: "bool \<Rightarrow> 'a \<Rightarrow> 'a \<Rightarrow> 'a" where
-[uexpr_defs]: "uIf = If"
 
-abbreviation cond ::
-  "('a,'\<alpha>) uexpr \<Rightarrow> (bool, '\<alpha>) uexpr \<Rightarrow> ('a,'\<alpha>) uexpr \<Rightarrow> ('a,'\<alpha>) uexpr"
-  ("(3_ \<triangleleft> _ \<triangleright>/ _)" [52,0,53] 52)
-  where "P \<triangleleft> b \<triangleright> Q \<equiv> trop uIf b P Q"
 
-definition eq_upred :: "('a, '\<alpha>) uexpr \<Rightarrow> ('a, '\<alpha>) uexpr \<Rightarrow> (bool, '\<alpha>) uexpr" (infixl "=\<^sub>u" 50)
-where [uexpr_defs]: "eq_upred x y = bop HOL.eq x y"
+
+text \<open>???????????????\<close>
 
 syntax
   "_uuvar" :: "svar \<Rightarrow> logic" ("_")
@@ -65,7 +53,7 @@ translations
 
 
 subsection \<open> Type class instantiations \<close>
-
+text \<open> Type class instantiations\<close>
   
 instantiation uexpr :: (zero, type) zero
 begin
@@ -91,179 +79,12 @@ begin
 instance ..
 end
 
-instantiation uexpr :: (minus, type) minus
-begin
-  definition minus_uexpr_def [uexpr_defs]: "u - v = bop (-) u v"
-instance ..
-end
-
-instantiation uexpr :: (times, type) times
-begin
-  definition times_uexpr_def [uexpr_defs]: "u * v = bop times u v"
-instance ..
-end
-
-instantiation uexpr :: (divide, type) divide
-begin
-  definition divide_uexpr :: "('a, 'b) uexpr \<Rightarrow> ('a, 'b) uexpr \<Rightarrow> ('a, 'b) uexpr" where
-  [uexpr_defs]: "divide_uexpr u v = bop divide u v"
-instance ..
-end
-
-instantiation uexpr :: (inverse, type) inverse
-begin
-  definition inverse_uexpr :: "('a, 'b) uexpr \<Rightarrow> ('a, 'b) uexpr"
-  where [uexpr_defs]: "inverse_uexpr u = uop inverse u"
-instance ..
-end
-
-instantiation uexpr :: (modulo, type) modulo
-begin
-  definition mod_uexpr_def [uexpr_defs]: "u mod v = bop (mod) u v"
-instance ..
-end
-
-
-
-
-
-
-instance uexpr :: (Rings.dvd, type) Rings.dvd ..
-
-instance uexpr :: (semigroup_add, type) semigroup_add
-  by (intro_classes) (simp add: plus_uexpr_def zero_uexpr_def, transfer, simp add: add.assoc)+
-
 instance uexpr :: (numeral, type) numeral
   by (intro_classes, simp add: plus_uexpr_def, transfer, simp add: add.assoc)
 
-instance uexpr :: (semigroup_mult, type) semigroup_mult
-  by (intro_classes) (simp add: times_uexpr_def one_uexpr_def, transfer, simp add: mult.assoc)+
-
-instance uexpr :: (monoid_mult, type) monoid_mult
-  by (intro_classes) (simp add: times_uexpr_def one_uexpr_def, transfer, simp)+
-
-instance uexpr :: (monoid_add, type) monoid_add
-  by (intro_classes) (simp add: plus_uexpr_def zero_uexpr_def, transfer, simp)+
-
-instance uexpr :: (ab_semigroup_add, type) ab_semigroup_add
-  by (intro_classes) (simp add: plus_uexpr_def, transfer, simp add: add.commute)+
-
-instance uexpr :: (cancel_semigroup_add, type) cancel_semigroup_add
-  by (intro_classes) (simp add: plus_uexpr_def, transfer, simp add: fun_eq_iff)+
-
-instance uexpr :: (cancel_ab_semigroup_add, type) cancel_ab_semigroup_add
-  by (intro_classes, (simp add: plus_uexpr_def minus_uexpr_def, transfer, simp add: fun_eq_iff add.commute cancel_ab_semigroup_add_class.diff_diff_add)+)
-
-instance uexpr :: (group_add, type) group_add
-  by (intro_classes)
-     (simp add: plus_uexpr_def uminus_uexpr_def minus_uexpr_def zero_uexpr_def, transfer, simp)+
-
-instance uexpr :: (ab_group_add, type) ab_group_add
-  by (intro_classes)
-     (simp add: plus_uexpr_def uminus_uexpr_def minus_uexpr_def zero_uexpr_def, transfer, simp)+
-
-instance uexpr :: (semiring, type) semiring
-  by (intro_classes) (simp add: plus_uexpr_def times_uexpr_def, transfer, simp add: fun_eq_iff add.commute semiring_class.distrib_right semiring_class.distrib_left)+
-
-instance uexpr :: (ring_1, type) ring_1
-  by (intro_classes) (simp add: plus_uexpr_def uminus_uexpr_def minus_uexpr_def times_uexpr_def zero_uexpr_def one_uexpr_def, transfer, simp add: fun_eq_iff)+
-
-
-
-
-
-
-lemma power_rep_eq: "\<lbrakk>P ^ n\<rbrakk>\<^sub>e = (\<lambda> b. \<lbrakk>P\<rbrakk>\<^sub>e b ^ n)"
-  by (induct n, simp_all add: lit.rep_eq one_uexpr_def bop.rep_eq times_uexpr_def)
-
-lemma lit_uminus [lit_simps]: "\<guillemotleft>- x\<guillemotright> = - \<guillemotleft>x\<guillemotright>" by (simp add: uexpr_defs, transfer, simp)
-lemma lit_minus [lit_simps]: "\<guillemotleft>x - y\<guillemotright> = \<guillemotleft>x\<guillemotright> - \<guillemotleft>y\<guillemotright>" by (simp add: uexpr_defs, transfer, simp)
-lemma lit_times [lit_simps]: "\<guillemotleft>x * y\<guillemotright> = \<guillemotleft>x\<guillemotright> * \<guillemotleft>y\<guillemotright>" by (simp add: uexpr_defs, transfer, simp)
-lemma lit_divide [lit_simps]: "\<guillemotleft>x / y\<guillemotright> = \<guillemotleft>x\<guillemotright> / \<guillemotleft>y\<guillemotright>" by (simp add: uexpr_defs, transfer, simp)
-lemma lit_div [lit_simps]: "\<guillemotleft>x div y\<guillemotright> = \<guillemotleft>x\<guillemotright> div \<guillemotleft>y\<guillemotright>" by (simp add: uexpr_defs, transfer, simp)
-lemma lit_power [lit_simps]: "\<guillemotleft>x ^ n\<guillemotright> = \<guillemotleft>x\<guillemotright> ^ n" by (simp add: lit.rep_eq power_rep_eq uexpr_eq_iff)
-
-
-                                                              
-
-subsection \<open> Syntax translations \<close>
-
-
-abbreviation (input) "ulens_override x f g \<equiv> lens_override f g x"
-
-definition set_of :: "'a itself \<Rightarrow> 'a set" where
-[uexpr_defs]: "set_of t = UNIV"
-
-nonterminal utuple_args and umaplet and umaplets
-
-syntax \<comment> \<open> Core expression constructs \<close>
-  "_ucoerce"    :: "logic \<Rightarrow> type \<Rightarrow> logic" (infix ":\<^sub>u" 50)
-  "_ulambda"    :: "pttrn \<Rightarrow> logic \<Rightarrow> logic" ("\<lambda> _ \<bullet> _" [0, 10] 10)
-  "_ulens_ovrd" :: "logic \<Rightarrow> logic \<Rightarrow> salpha \<Rightarrow> logic" ("_ \<oplus> _ on _" [85, 0, 86] 86)
-  "_ulens_get"  :: "logic \<Rightarrow> svar \<Rightarrow> logic" ("_:_" [900,901] 901)
-  "_umem"       :: "('a, '\<alpha>) uexpr \<Rightarrow> ('a set, '\<alpha>) uexpr \<Rightarrow> (bool, '\<alpha>) uexpr" (infix "\<in>\<^sub>u" 50)
-
-translations
-  "\<lambda> x \<bullet> p" == "CONST ulambda (\<lambda> x. p)"
-  "x :\<^sub>u 'a" == "x :: ('a, _) uexpr"
-  "_ulens_ovrd f g a" => "CONST bop (CONST ulens_override a) f g"
-  "_ulens_ovrd f g a" <= "CONST bop (\<lambda>x y. CONST lens_override x1 y1 a) f g"
-  "_ulens_get x y" == "CONST uop (CONST lens_get y) x"
-  "x \<in>\<^sub>u A" == "CONST bop (\<in>) x A"
-
-syntax \<comment> \<open> Tuples \<close>
-  "_utuple"     :: "('a, '\<alpha>) uexpr \<Rightarrow> utuple_args \<Rightarrow> ('a * 'b, '\<alpha>) uexpr" ("(1'(_,/ _')\<^sub>u)")
-  "_utuple_arg"  :: "('a, '\<alpha>) uexpr \<Rightarrow> utuple_args" ("_")
-  "_utuple_args" :: "('a, '\<alpha>) uexpr => utuple_args \<Rightarrow> utuple_args"     ("_,/ _")
-  "_uunit"      :: "('a, '\<alpha>) uexpr" ("'(')\<^sub>u")
-  "_ufst"       :: "('a \<times> 'b, '\<alpha>) uexpr \<Rightarrow> ('a, '\<alpha>) uexpr" ("\<pi>\<^sub>1'(_')")
-  "_usnd"       :: "('a \<times> 'b, '\<alpha>) uexpr \<Rightarrow> ('b, '\<alpha>) uexpr" ("\<pi>\<^sub>2'(_')")
-
-translations
-  "()\<^sub>u"      == "\<guillemotleft>()\<guillemotright>"
-  "(x, y)\<^sub>u"  == "CONST bop (CONST Pair) x y"
-  "_utuple x (_utuple_args y z)" == "_utuple x (_utuple_arg (_utuple y z))"
-  "\<pi>\<^sub>1(x)"    == "CONST uop CONST fst x"
-  "\<pi>\<^sub>2(x)"    == "CONST uop CONST snd x"
-
-
-
-
-
-
-
-subsection \<open> Evaluation laws for expressions \<close>
-
-
-
-
-lemma lit_ueval [ueval]: "\<lbrakk>\<guillemotleft>x\<guillemotright>\<rbrakk>\<^sub>eb = x"
-  by (transfer, simp)
-lemma var_ueval [ueval]: "\<lbrakk>var x\<rbrakk>\<^sub>eb = get\<^bsub>x\<^esub> b"
-  by (transfer, simp)
-lemma uop_ueval [ueval]: "\<lbrakk>uop f x\<rbrakk>\<^sub>eb = f (\<lbrakk>x\<rbrakk>\<^sub>eb)"
-  by (transfer, simp)
-lemma bop_ueval [ueval]: "\<lbrakk>bop f x y\<rbrakk>\<^sub>eb = f (\<lbrakk>x\<rbrakk>\<^sub>eb) (\<lbrakk>y\<rbrakk>\<^sub>eb)"
-  by (transfer, simp)
-lemma trop_ueval [ueval]: "\<lbrakk>trop f x y z\<rbrakk>\<^sub>eb = f (\<lbrakk>x\<rbrakk>\<^sub>eb) (\<lbrakk>y\<rbrakk>\<^sub>eb) (\<lbrakk>z\<rbrakk>\<^sub>eb)"
-  by (transfer, simp)
-
-lemma uop_const [simp]: "uop id u = u"
-  by (transfer, simp)
-lemma bop_const_1 [simp]: "bop (\<lambda>x y. y) u v = v"
-  by (transfer, simp)
-lemma bop_const_2 [simp]: "bop (\<lambda>x y. x) u v = u"
-  by (transfer, simp)
-
-
-
-
-
-
 lemma lit_fun_simps [lit_simps]:
-  "\<guillemotleft>h x y z\<guillemotright> = trop h \<guillemotleft>x\<guillemotright> \<guillemotleft>y\<guillemotright> \<guillemotleft>z\<guillemotright>"
-  "\<guillemotleft>g x y\<guillemotright> = bop g \<guillemotleft>x\<guillemotright> \<guillemotleft>y\<guillemotright>"
   "\<guillemotleft>f x\<guillemotright> = uop f \<guillemotleft>x\<guillemotright>"
+  "\<guillemotleft>g x y\<guillemotright> = bop g \<guillemotleft>x\<guillemotright> \<guillemotleft>y\<guillemotright>"
   by (transfer, simp)+
 
 lemma numeral_uexpr_rep_eq: "\<lbrakk>numeral x\<rbrakk>\<^sub>e b = numeral x"
@@ -288,6 +109,23 @@ lemma lit_numeral [lit_simps]: "\<guillemotleft>numeral n\<guillemotright> = num
 
 
 
+subsection \<open> Evaluation laws for expressions \<close>
+
+lemma lit_ueval [ueval]: "\<lbrakk>\<guillemotleft>x\<guillemotright>\<rbrakk>\<^sub>eb = x"
+  by (transfer, simp)
+lemma var_ueval [ueval]: "\<lbrakk>var x\<rbrakk>\<^sub>eb = get\<^bsub>x\<^esub> b"
+  by (transfer, simp)
+lemma uop_ueval [ueval]: "\<lbrakk>uop f x\<rbrakk>\<^sub>eb = f (\<lbrakk>x\<rbrakk>\<^sub>eb)"
+  by (transfer, simp)
+lemma bop_ueval [ueval]: "\<lbrakk>bop f x y\<rbrakk>\<^sub>eb = f (\<lbrakk>x\<rbrakk>\<^sub>eb) (\<lbrakk>y\<rbrakk>\<^sub>eb)"
+  by (transfer, simp)
+lemma uop_const [simp]: "uop id u = u"
+  by (transfer, simp)
+lemma bop_const_1 [simp]: "bop (\<lambda>x y. y) u v = v"
+  by (transfer, simp)
+lemma bop_const_2 [simp]: "bop (\<lambda>x y. x) u v = u"
+  by (transfer, simp)
+
 lemma lit_numeral_1: "uop numeral x = Abs_uexpr (\<lambda>b. numeral (\<lbrakk>x\<rbrakk>\<^sub>e b))"
   by (simp add: uop_def)
 
@@ -298,362 +136,13 @@ method literalise = (unfold lit_simps[THEN sym])
 method unliteralise = (unfold lit_simps uexpr_defs[THEN sym];
                      (unfold lit_numeral_1 ; (unfold uexpr_defs ueval); (unfold lit_numeral_2))?)+
 
-
-
-
 method uexpr_simp uses simps = ((literalise)?, simp add: lit_norm simps, (unliteralise)?)
 
 (* Example *)
-  
 lemma "((1::(int, '\<alpha>) uexpr) + \<guillemotleft>2\<guillemotright> = 4) = (\<guillemotleft>3\<guillemotright> = 4)"
   apply (literalise)
   apply (uexpr_simp) oops
 
-
-
-
-
-
-
-
-
-
-
-
-
-
-
-subsection \<open> Syntax translations about functions \<close>
-
-(***  utp-expr-funcs.thy    ***)
-
-
-
-syntax \<comment> \<open> Polymorphic constructs \<close>
-  "_uceil"      :: "logic \<Rightarrow> logic" ("\<lceil>_\<rceil>\<^sub>u")
-  "_ufloor"     :: "logic \<Rightarrow> logic" ("\<lfloor>_\<rfloor>\<^sub>u")
-  "_umin"       :: "logic \<Rightarrow> logic \<Rightarrow> logic" ("min\<^sub>u'(_, _')")
-  "_umax"       :: "logic \<Rightarrow> logic \<Rightarrow> logic" ("max\<^sub>u'(_, _')")
-  "_ugcd"       :: "logic \<Rightarrow> logic \<Rightarrow> logic" ("gcd\<^sub>u'(_, _')")
-
-translations
-  \<comment> \<open> Type-class polymorphic constructs \<close>
-  "min\<^sub>u(x, y)"  == "CONST bop (CONST min) x y"
-  "max\<^sub>u(x, y)"  == "CONST bop (CONST max) x y"
-  "gcd\<^sub>u(x, y)"  == "CONST bop (CONST gcd) x y"
-  "\<lceil>x\<rceil>\<^sub>u" == "CONST uop CONST ceiling x"
-  "\<lfloor>x\<rfloor>\<^sub>u" == "CONST uop CONST floor x"
-
-syntax \<comment> \<open> Lists / Sequences \<close>
-  "_ucons"      :: "logic \<Rightarrow> logic \<Rightarrow> logic" (infixr "#\<^sub>u" 65)
-  "_unil"       :: "('a list, '\<alpha>) uexpr" ("\<langle>\<rangle>")
-  "_ulist"      :: "args => ('a list, '\<alpha>) uexpr"    ("\<langle>(_)\<rangle>")
-  "_uappend"    :: "('a list, '\<alpha>) uexpr \<Rightarrow> ('a list, '\<alpha>) uexpr \<Rightarrow> ('a list, '\<alpha>) uexpr" (infixr "^\<^sub>u" 80)
-  "_udconcat"   :: "logic \<Rightarrow> logic \<Rightarrow> logic" (infixr "\<^sup>\<frown>\<^sub>u" 90)
-  "_ulast"      :: "('a list, '\<alpha>) uexpr \<Rightarrow> ('a, '\<alpha>) uexpr" ("last\<^sub>u'(_')")
-  "_ufront"     :: "('a list, '\<alpha>) uexpr \<Rightarrow> ('a list, '\<alpha>) uexpr" ("front\<^sub>u'(_')")
-  "_uhead"      :: "('a list, '\<alpha>) uexpr \<Rightarrow> ('a, '\<alpha>) uexpr" ("head\<^sub>u'(_')")
-  "_utail"      :: "('a list, '\<alpha>) uexpr \<Rightarrow> ('a list, '\<alpha>) uexpr" ("tail\<^sub>u'(_')")
-  "_utake"      :: "(nat, '\<alpha>) uexpr \<Rightarrow> ('a list, '\<alpha>) uexpr \<Rightarrow> ('a list, '\<alpha>) uexpr" ("take\<^sub>u'(_,/ _')")
-  "_udrop"      :: "(nat, '\<alpha>) uexpr \<Rightarrow> ('a list, '\<alpha>) uexpr \<Rightarrow> ('a list, '\<alpha>) uexpr" ("drop\<^sub>u'(_,/ _')")
-  "_ufilter"    :: "('a list, '\<alpha>) uexpr \<Rightarrow> ('a set, '\<alpha>) uexpr \<Rightarrow> ('a list, '\<alpha>) uexpr" (infixl "\<restriction>\<^sub>u" 75)
-  "_uextract"   :: "('a set, '\<alpha>) uexpr \<Rightarrow> ('a list, '\<alpha>) uexpr \<Rightarrow> ('a list, '\<alpha>) uexpr" (infixl "\<upharpoonleft>\<^sub>u" 75)
-  "_uelems"     :: "('a list, '\<alpha>) uexpr \<Rightarrow> ('a set, '\<alpha>) uexpr" ("elems\<^sub>u'(_')")
-  "_usorted"    :: "('a list, '\<alpha>) uexpr \<Rightarrow> (bool, '\<alpha>) uexpr" ("sorted\<^sub>u'(_')")
-  "_udistinct"  :: "('a list, '\<alpha>) uexpr \<Rightarrow> (bool, '\<alpha>) uexpr" ("distinct\<^sub>u'(_')")
-  "_uupto"      :: "logic \<Rightarrow> logic \<Rightarrow> logic" ("\<langle>_.._\<rangle>")
-  "_uupt"       :: "logic \<Rightarrow> logic \<Rightarrow> logic" ("\<langle>_..<_\<rangle>")
-  "_umap"       :: "logic \<Rightarrow> logic \<Rightarrow> logic" ("map\<^sub>u")
-  "_uzip"       :: "logic \<Rightarrow> logic \<Rightarrow> logic" ("zip\<^sub>u")
-
-subsection \<open> Distributed Concatenation \<close>
-
-definition uncurry :: "('a \<Rightarrow> 'b \<Rightarrow>  'c) \<Rightarrow> ('a \<times> 'b \<Rightarrow> 'c)" where
-[simp]: "uncurry f = (\<lambda>(x, y). f x y)"
-
-definition dist_concat ::
-  "'a list set \<Rightarrow> 'a list set \<Rightarrow> 'a list set" (infixr "\<^sup>\<frown>" 100) where
-"dist_concat ls1 ls2 = (uncurry (@) ` (ls1 \<times> ls2))"
-
-subsection \<open> Filtering a list according to a set \<close>
-
-definition seq_filter :: "'a list \<Rightarrow> 'a set \<Rightarrow> 'a list" (infix "\<restriction>\<^sub>l" 80) where
-"seq_filter xs A = filter (\<lambda> x. x \<in> A) xs"
-
-subsection \<open> Extracting List Elements \<close>
-
-definition seq_extract :: "nat set \<Rightarrow> 'a list \<Rightarrow> 'a list" (infix "\<upharpoonleft>\<^sub>l" 80) where
-"seq_extract A xs = nths xs A"
-
-translations
-  "x #\<^sub>u ys" == "CONST bop (#) x ys"
-  "\<langle>\<rangle>"       == "\<guillemotleft>[]\<guillemotright>"
-  "\<langle>x, xs\<rangle>"  == "x #\<^sub>u \<langle>xs\<rangle>"
-  "\<langle>x\<rangle>"      == "x #\<^sub>u \<guillemotleft>[]\<guillemotright>"
-  "x ^\<^sub>u y"   == "CONST bop (@) x y"
-  "A \<^sup>\<frown>\<^sub>u B" == "CONST bop (\<^sup>\<frown>) A B"
-  "last\<^sub>u(xs)" == "CONST uop CONST last xs"
-  "front\<^sub>u(xs)" == "CONST uop CONST butlast xs"
-  "head\<^sub>u(xs)" == "CONST uop CONST hd xs"
-  "tail\<^sub>u(xs)" == "CONST uop CONST tl xs"
-  "drop\<^sub>u(n,xs)" == "CONST bop CONST drop n xs"
-  "take\<^sub>u(n,xs)" == "CONST bop CONST take n xs"
-  "elems\<^sub>u(xs)" == "CONST uop CONST set xs"
-  "sorted\<^sub>u(xs)" == "CONST uop CONST sorted xs"
-  "distinct\<^sub>u(xs)" == "CONST uop CONST distinct xs"
-  "xs \<restriction>\<^sub>u A"   == "CONST bop CONST seq_filter xs A"
-  "A \<upharpoonleft>\<^sub>u xs"   == "CONST bop (\<upharpoonleft>\<^sub>l) A xs"
-  "\<langle>n..k\<rangle>" == "CONST bop CONST upto n k"
-  "\<langle>n..<k\<rangle>" == "CONST bop CONST upt n k"
-  "map\<^sub>u f xs" == "CONST bop CONST map f xs"
-  "zip\<^sub>u xs ys" == "CONST bop CONST zip xs ys"
-
-syntax \<comment> \<open> Sets \<close>
-  "_ufinite"    :: "logic \<Rightarrow> logic" ("finite\<^sub>u'(_')")
-  "_uempset"    :: "('a set, '\<alpha>) uexpr" ("{}\<^sub>u")
-  "_uset"       :: "args => ('a set, '\<alpha>) uexpr" ("{(_)}\<^sub>u")
-  "_uunion"     :: "('a set, '\<alpha>) uexpr \<Rightarrow> ('a set, '\<alpha>) uexpr \<Rightarrow> ('a set, '\<alpha>) uexpr" (infixl "\<union>\<^sub>u" 65)
-  "_uinter"     :: "('a set, '\<alpha>) uexpr \<Rightarrow> ('a set, '\<alpha>) uexpr \<Rightarrow> ('a set, '\<alpha>) uexpr" (infixl "\<inter>\<^sub>u" 70)
-  "_uinsert"    :: "logic \<Rightarrow> logic \<Rightarrow> logic" ("insert\<^sub>u")
-  "_uimage"     :: "logic \<Rightarrow> logic \<Rightarrow> logic" ("_\<lparr>_\<rparr>\<^sub>u" [10,0] 10)
-  "_usubset"    :: "('a set, '\<alpha>) uexpr \<Rightarrow> ('a set, '\<alpha>) uexpr \<Rightarrow> (bool, '\<alpha>) uexpr" (infix "\<subset>\<^sub>u" 50)
-  "_usubseteq"  :: "('a set, '\<alpha>) uexpr \<Rightarrow> ('a set, '\<alpha>) uexpr \<Rightarrow> (bool, '\<alpha>) uexpr" (infix "\<subseteq>\<^sub>u" 50)
-  "_uconverse"  :: "logic \<Rightarrow> logic" ("(_\<^sup>~)" [1000] 999)
-  "_ucarrier"   :: "type \<Rightarrow> logic" ("[_]\<^sub>T")
-  "_uid"        :: "type \<Rightarrow> logic" ("id[_]")
-  "_uproduct"   :: "logic \<Rightarrow> logic \<Rightarrow> logic" (infixr "\<times>\<^sub>u" 80)
-  "_urelcomp"   :: "logic \<Rightarrow> logic \<Rightarrow> logic" (infixr ";\<^sub>u" 75)
-
-translations
-  "finite\<^sub>u(x)" == "CONST uop (CONST finite) x"
-  "{}\<^sub>u"      == "\<guillemotleft>{}\<guillemotright>"
-  "insert\<^sub>u x xs" == "CONST bop CONST insert x xs"
-  "{x, xs}\<^sub>u" == "insert\<^sub>u x {xs}\<^sub>u"
-  "{x}\<^sub>u"     == "insert\<^sub>u x \<guillemotleft>{}\<guillemotright>"
-  "A \<union>\<^sub>u B"   == "CONST bop (\<union>) A B"
-  "A \<inter>\<^sub>u B"   == "CONST bop (\<inter>) A B"
-  "f\<lparr>A\<rparr>\<^sub>u"     == "CONST bop CONST image f A"
-  "A \<subset>\<^sub>u B"   == "CONST bop (\<subset>) A B"
-
-
-  "A \<subseteq>\<^sub>u B"   == "CONST bop (\<subseteq>) A B"
-
-
-  "P\<^sup>~"        == "CONST uop CONST converse P"
-  "['a]\<^sub>T"     == "\<guillemotleft>CONST set_of TYPE('a)\<guillemotright>"
-  "id['a]"    == "\<guillemotleft>CONST Id_on (CONST set_of TYPE('a))\<guillemotright>"
-  "A \<times>\<^sub>u B"    == "CONST bop CONST Product_Type.Times A B"
-  "A ;\<^sub>u B"    == "CONST bop CONST relcomp A B"
-
-syntax \<comment> \<open> Partial functions \<close>
-  "_umap_plus"  :: "logic \<Rightarrow> logic \<Rightarrow> logic" (infixl "\<oplus>\<^sub>u" 85)
-  "_umap_minus" :: "logic \<Rightarrow> logic \<Rightarrow> logic" (infixl "\<ominus>\<^sub>u" 85)
-
-typedef ('a, 'b) pfun = "UNIV :: ('a \<rightharpoonup> 'b) set" ..
-
-translations
-  "f \<oplus>\<^sub>u g"   => "(f :: ((_, _) pfun, _) uexpr) + g"
-  "f \<ominus>\<^sub>u g"   => "(f :: ((_, _) pfun, _) uexpr) - g"
-  
-syntax \<comment> \<open> Sum types \<close>
-  "_uinl"       :: "logic \<Rightarrow> logic" ("inl\<^sub>u'(_')")
-  "_uinr"       :: "logic \<Rightarrow> logic" ("inr\<^sub>u'(_')")
-  
-translations
-  "inl\<^sub>u(x)" == "CONST uop CONST Inl x"
-  "inr\<^sub>u(x)" == "CONST uop CONST Inr x"
-
-
-
-
-
-(***   utp_unrest.thy   unrestriction   ***)
-
-
-
-subsection \<open> Unrestriction Definitions and Core Syntax \<close>
-  
-text \<open> Unrestriction is an encoding of semantic freshness that allows us to reason about the
-  presence of variables in predicates without being concerned with abstract syntax trees.
-  An expression $p$ is unrestricted by lens $x$, written $x \mathop{\sharp} p$, if
-  altering the value of $x$ has no effect on the valuation of $p$. This is a sufficient
-  notion to prove many laws that would ordinarily rely on an \emph{fv} function. 
-
-  Unrestriction was first defined in the work of Marcel Oliveira~\cite{Oliveira2005-PHD,Oliveira07} in his
-  UTP mechanisation in \emph{ProofPowerZ}. Our definition modifies his in that our variables
-  are semantically characterised as lenses, and supported by the lens laws, rather than named 
-  syntactic entities. We effectively fuse the ideas from both Feliachi~\cite{Feliachi2010} and 
-  Oliveira's~\cite{Oliveira07} mechanisations of the UTP, the former being also purely semantic
-  in nature.
-
-  We first set up overloaded syntax for unrestriction, as several concepts will have this
-  defined. \<close>
-
-consts
-  unrest :: "'a \<Rightarrow> 'b \<Rightarrow> bool"
-syntax
-  "_unrest" :: "salpha \<Rightarrow> logic \<Rightarrow> logic \<Rightarrow> logic" (infix "\<sharp>" 20)
-translations
-  "_unrest x p" == "CONST unrest x p"                                           
-  "_unrest (_salphaset (_salphamk (x +\<^sub>L y))) P"  <= "_unrest (x +\<^sub>L y) P"
-
-named_theorems unrest
-method unrest_tac = (simp add: unrest)?
-  
-lift_definition unrest_uexpr :: "('a \<Longrightarrow> '\<alpha>) \<Rightarrow> ('b, '\<alpha>) uexpr \<Rightarrow> bool"
-is "\<lambda> x e. \<forall> b v. e (put\<^bsub>x\<^esub> b v) = e b" .
-
-adhoc_overloading
-  unrest unrest_uexpr
-
-lemma unrest_expr_alt_def:
-  "weak_lens x \<Longrightarrow> (x \<sharp> P) = (\<forall> b b'. \<lbrakk>P\<rbrakk>\<^sub>e (b \<oplus>\<^sub>L b' on x) = \<lbrakk>P\<rbrakk>\<^sub>e b)"
-  by (transfer, metis lens_override_def weak_lens.put_get)
-  
-subsection \<open> Unrestriction laws \<close>
-
-lemma unrest_var_comp [unrest]:
-  "\<lbrakk> x \<sharp> P; y \<sharp> P \<rbrakk> \<Longrightarrow> x;y \<sharp> P"
-  by (transfer, simp add: lens_defs)
-
-lemma unrest_svar [unrest]: "(&x \<sharp> P) \<longleftrightarrow> (x \<sharp> P)"
-  by (transfer, simp add: lens_defs)
-
-text \<open> No lens is restricted by a literal, since it returns the same value for any state binding. \<close>
-    
-lemma unrest_lit [unrest]: "x \<sharp> \<guillemotleft>v\<guillemotright>"
-  by (transfer, simp)
-
-text \<open> If one lens is smaller than another, then any unrestriction on the larger lens implies
-  unrestriction on the smaller. \<close>
-    
-lemma unrest_sublens:
-  fixes P :: "('a, '\<alpha>) uexpr"
-  assumes "x \<sharp> P" "y \<subseteq>\<^sub>L x"
-  shows "y \<sharp> P" 
-  using assms
-  by (transfer, metis (no_types, lifting) lens.select_convs(2) lens_comp_def sublens_def)
-    
-text \<open> If two lenses are equivalent, and thus they characterise the same state-space regions,
-  then clearly unrestrictions over them are equivalent. \<close>
-    
-lemma unrest_equiv:
-  fixes P :: "('a, '\<alpha>) uexpr"
-  assumes "mwb_lens y" "x \<approx>\<^sub>L y" "x \<sharp> P"
-  shows "y \<sharp> P"
-  by (metis assms lens_equiv_def sublens_pres_mwb sublens_put_put unrest_uexpr.rep_eq)
-
-text \<open> If we can show that an expression is unrestricted on a bijective lens, then is unrestricted
-  on the entire state-space. \<close>
-
-lemma bij_lens_unrest_all:
-  fixes P :: "('a, '\<alpha>) uexpr"
-  assumes "bij_lens X" "X \<sharp> P"
-  shows "\<Sigma> \<sharp> P"
-  using assms bij_lens_equiv_id lens_equiv_def unrest_sublens by blast
-
-lemma bij_lens_unrest_all_eq:
-  fixes P :: "('a, '\<alpha>) uexpr"
-  assumes "bij_lens X"
-  shows "(\<Sigma> \<sharp> P) \<longleftrightarrow> (X \<sharp> P)"
-  by (meson assms bij_lens_equiv_id lens_equiv_def unrest_sublens)
-
-text \<open> If an expression is unrestricted by all variables, then it is unrestricted by any variable \<close>
-
-lemma unrest_all_var:
-  fixes e :: "('a, '\<alpha>) uexpr"
-  assumes "\<Sigma> \<sharp> e"
-  shows "x \<sharp> e"
-  by (metis assms id_lens_def lens.simps(2) unrest_uexpr.rep_eq)
-
-text \<open> We can split an unrestriction composed by lens plus \<close>
-
-lemma unrest_plus_split:
-  fixes P :: "('a, '\<alpha>) uexpr"
-  assumes "x \<bowtie> y" "vwb_lens x" "vwb_lens y"
-  shows "unrest (x +\<^sub>L y) P \<longleftrightarrow> (x \<sharp> P) \<and> (y \<sharp> P)"
-  using assms
-  by (meson lens_plus_right_sublens lens_plus_ub sublens_refl unrest_sublens unrest_var_comp vwb_lens_wb)
-
-text \<open> The following laws demonstrate the primary motivation for lens independence: a variable
-  expression is unrestricted by another variable only when the two variables are independent. 
-  Lens independence thus effectively allows us to semantically characterise when two variables,
-  or sets of variables, are different. \<close>
-
-lemma unrest_var [unrest]: "\<lbrakk> mwb_lens x; x \<bowtie> y \<rbrakk> \<Longrightarrow> y \<sharp> var x"
-  by (transfer, auto)
-    
-lemma unrest_iuvar [unrest]: "\<lbrakk> mwb_lens x; x \<bowtie> y \<rbrakk> \<Longrightarrow> $y \<sharp> $x"
-  by (simp add: unrest_var)
-
-lemma unrest_ouvar [unrest]: "\<lbrakk> mwb_lens x; x \<bowtie> y \<rbrakk> \<Longrightarrow> $y\<acute> \<sharp> $x\<acute>"
-  by (simp add: unrest_var)
-
-text \<open> The following laws follow automatically from independence of input and output variables. \<close>
-    
-lemma unrest_iuvar_ouvar [unrest]:
-  fixes x :: "('a \<Longrightarrow> '\<alpha>)"
-  assumes "mwb_lens y"
-  shows "$x \<sharp> $y\<acute>"
-  by (metis prod.collapse unrest_uexpr.rep_eq var.rep_eq var_lookup_out var_update_in)
-
-lemma unrest_ouvar_iuvar [unrest]:
-  fixes x :: "('a \<Longrightarrow> '\<alpha>)"
-  assumes "mwb_lens y"
-  shows "$x\<acute> \<sharp> $y"
-  by (metis prod.collapse unrest_uexpr.rep_eq var.rep_eq var_lookup_in var_update_out)
-
-text \<open> Unrestriction distributes through the various function lifting expression constructs;
-  this allows us to prove unrestrictions for the majority of the expression language. \<close>
-    
-lemma unrest_uop [unrest]: "x \<sharp> e \<Longrightarrow> x \<sharp> uop f e"
-  by (transfer, simp)
-
-lemma unrest_bop [unrest]: "\<lbrakk> x \<sharp> u; x \<sharp> v \<rbrakk> \<Longrightarrow> x \<sharp> bop f u v"
-  by (transfer, simp)
-
-lemma unrest_trop [unrest]: "\<lbrakk> x \<sharp> u; x \<sharp> v; x \<sharp> w \<rbrakk> \<Longrightarrow> x \<sharp> trop f u v w"
-  by (transfer, simp)
-
-text \<open> For convenience, we also prove unrestriction rules for the bespoke operators on equality,
-  numbers, arithmetic etc. \<close>
-    
-lemma unrest_eq [unrest]: "\<lbrakk> x \<sharp> u; x \<sharp> v \<rbrakk> \<Longrightarrow> x \<sharp> u =\<^sub>u v"
-  by (simp add: eq_upred_def, transfer, simp)
-
-lemma unrest_zero [unrest]: "x \<sharp> 0"
-  by (simp add: unrest_lit zero_uexpr_def)
-
-lemma unrest_one [unrest]: "x \<sharp> 1"
-  by (simp add: one_uexpr_def unrest_lit)
-
-lemma unrest_numeral [unrest]: "x \<sharp> (numeral n)"
-  by (simp add: numeral_uexpr_simp unrest_lit)
-
-lemma unrest_plus [unrest]: "\<lbrakk> x \<sharp> u; x \<sharp> v \<rbrakk> \<Longrightarrow> x \<sharp> u + v"
-  by (simp add: plus_uexpr_def unrest)
-
-lemma unrest_uminus [unrest]: "x \<sharp> u \<Longrightarrow> x \<sharp> - u"
-  by (simp add: uminus_uexpr_def unrest)
-
-lemma unrest_minus [unrest]: "\<lbrakk> x \<sharp> u; x \<sharp> v \<rbrakk> \<Longrightarrow> x \<sharp> u - v"
-  by (simp add: minus_uexpr_def unrest)
-
-lemma unrest_times [unrest]: "\<lbrakk> x \<sharp> u; x \<sharp> v \<rbrakk> \<Longrightarrow> x \<sharp> u * v"
-  by (simp add: times_uexpr_def unrest)
-
-lemma unrest_divide [unrest]: "\<lbrakk> x \<sharp> u; x \<sharp> v \<rbrakk> \<Longrightarrow> x \<sharp> u / v"
-  by (simp add: divide_uexpr_def unrest)
-
-lemma unrest_case_prod [unrest]: "\<lbrakk> \<And> i j. x \<sharp> P i j \<rbrakk> \<Longrightarrow> x \<sharp> case_prod P v"
-  by (simp add: prod.split_sel_asm)
-
-text \<open> For a $\lambda$-term we need to show that the characteristic function expression does
-  not restrict $v$ for any input value $x$. \<close>
-    
-lemma unrest_ulambda [unrest]:
-  "\<lbrakk> \<And> x. v \<sharp> F x \<rbrakk> \<Longrightarrow> v \<sharp> (\<lambda> x \<bullet> F x)"
-  by (transfer, simp)
 
 
 
@@ -671,9 +160,9 @@ named_theorems usubst
 type_synonym ('\<alpha>,'\<beta>) psubst = "'\<alpha> \<Rightarrow> '\<beta>"
 type_synonym '\<alpha> usubst = "'\<alpha> \<Rightarrow> '\<alpha>"
   
-lift_definition subst :: "('\<alpha>, '\<beta>) psubst \<Rightarrow> ('a, '\<beta>) uexpr \<Rightarrow> ('a, '\<alpha>) uexpr" is
+lift_definition subst :: " '\<alpha> usubst \<Rightarrow> ('a, '\<alpha>) uexpr \<Rightarrow> ('a, '\<alpha>) uexpr" is
 "\<lambda> \<sigma> e b. e (\<sigma> b)" .
-
+                    
 adhoc_overloading
   usubst subst
 
@@ -692,29 +181,13 @@ definition unrest_usubst :: "('a \<Longrightarrow> '\<alpha>) \<Rightarrow> '\<a
 where "unrest_usubst x \<sigma> = (\<forall> \<rho> v. \<sigma> (put\<^bsub>x\<^esub> \<rho> v) = put\<^bsub>x\<^esub> (\<sigma> \<rho>) v)"
 
 adhoc_overloading
-  unrest unrest_usubst
-  
-definition cond_subst :: "'\<alpha> usubst \<Rightarrow> (bool, '\<alpha>) uexpr \<Rightarrow> '\<alpha> usubst \<Rightarrow> '\<alpha> usubst" ("(3_ \<triangleleft> _ \<triangleright>\<^sub>s/ _)" [52,0,53] 52) where
-"cond_subst \<sigma> b \<rho> = (\<lambda> s. if \<lbrakk>b\<rbrakk>\<^sub>e s then \<sigma>(s) else \<rho>(s))"
+   unrest_usubst
   
 definition par_subst :: "'\<alpha> usubst \<Rightarrow> ('a \<Longrightarrow> '\<alpha>) \<Rightarrow> ('b \<Longrightarrow> '\<alpha>) \<Rightarrow> '\<alpha> usubst \<Rightarrow> '\<alpha> usubst" where
 "par_subst \<sigma>\<^sub>1 A B \<sigma>\<^sub>2 = (\<lambda> s. (s \<oplus>\<^sub>L (\<sigma>\<^sub>1 s) on A) \<oplus>\<^sub>L (\<sigma>\<^sub>2 s) on B)"
 
-
-
 subsection \<open> Syntax translations about subsitution \<close>
 
-text \<open> We support two kinds of syntax for substitutions, one where we construct a substitution
-  using a maplet-style syntax, with variables mapping to expressions. Such a constructed substitution
-  can be applied to an expression. Alternatively, we support the more traditional notation, 
-  $P \llbracket v / x \rrbracket$, which also support multiple simultaneous substitutions. We 
-  have to use double square brackets as the single ones are already well used. 
-
-  We set up non-terminals to represent a single substitution maplet, a sequence of maplets, a
-  list of expressions, and a list of alphabets. The parser effectively uses @{term subst_upd}
-  to construct substitutions from multiple variables. 
-\<close>
-  
 nonterminal smaplet and smaplets and uexp and uexprs and salphas
 
 syntax
@@ -724,32 +197,25 @@ syntax
   "_SubstUpd" :: "['m usubst, smaplets] => 'm usubst" ("_/'(_')" [900,0] 900)
   "_Subst"    :: "smaplets => 'a \<rightharpoonup> 'b"            ("(1[_])")
   "_psubst"  :: "[logic, svars, uexprs] \<Rightarrow> logic"
-  "_subst"   :: "logic \<Rightarrow> uexprs \<Rightarrow> salphas \<Rightarrow> logic" ("(_\<lbrakk>_'/_\<rbrakk>)" [990,0,0] 991)
+
   "_uexp_l"  :: "logic \<Rightarrow> uexp" ("_" [64] 64)
   "_uexprs"  :: "[uexp, uexprs] => uexprs" ("_,/ _")
   ""         :: "uexp => uexprs" ("_")
   "_salphas" :: "[salpha, salphas] => salphas" ("_,/ _")
   ""         :: "salpha => salphas" ("_")
-  "_par_subst" :: "logic \<Rightarrow> salpha \<Rightarrow> salpha \<Rightarrow> logic \<Rightarrow> logic" ("_ [_|_]\<^sub>s _" [100,0,0,101] 101)
-    
+
 translations
   "_SubstUpd m (_SMaplets xy ms)"     == "_SubstUpd (_SubstUpd m xy) ms"
   "_SubstUpd m (_smaplet x y)"        == "CONST subst_upd m x y"
   "_Subst ms"                         == "_SubstUpd (CONST id) ms"
   "_Subst (_SMaplets ms1 ms2)"        <= "_SubstUpd (_Subst ms1) ms2"
   "_SMaplets ms1 (_SMaplets ms2 ms3)" <= "_SMaplets (_SMaplets ms1 ms2) ms3"
-  "_subst P es vs" => "CONST subst (_psubst (CONST id) vs es) P"
   "_psubst m (_salphas x xs) (_uexprs v vs)" => "_psubst (_psubst m x v) xs vs"
   "_psubst m x v"  => "CONST subst_upd m x v"
-  "_subst P v x" <= "CONST usubst (CONST subst_upd (CONST id) x v) P"
-  "_subst P v x" <= "_subst P (_spvar x) v"
-  "_par_subst \<sigma>\<^sub>1 A B \<sigma>\<^sub>2" == "CONST par_subst \<sigma>\<^sub>1 A B \<sigma>\<^sub>2"
   "_uexp_l e" => "e"
 
 text \<open> Thus we can write things like @{term "\<sigma>(x \<mapsto>\<^sub>s v)"} to update a variable $x$ in $\sigma$ with
   expression $v$, @{term "[x \<mapsto>\<^sub>s e, y \<mapsto>\<^sub>s f]"} to construct a substitution with two variables,
-  and finally @{term "P\<lbrakk>v/x\<rbrakk>"}, the traditional syntax.
-
   We can now express deletion of a substitution maplet. \<close>
 
 definition subst_del :: "'\<alpha> usubst \<Rightarrow> ('a \<Longrightarrow> '\<alpha>) \<Rightarrow> '\<alpha> usubst" (infix "-\<^sub>s" 85) where
@@ -759,11 +225,10 @@ subsection \<open> Substitution Application Laws \<close>
 
 text \<open> We set up a simple substitution tactic that applies substitution and unrestriction laws \<close>
 
-method subst_tac = (simp add: usubst unrest)?
+method subst_tac = (simp add: usubst )?
 
 text \<open> Evaluation of a substitution expression involves application of the substitution to different
-  variables. Thus we first prove laws for these cases. The simplest substitution, $id$, when applied
-  to any variable $x$ simply returns the variable expression, since $id$ has no effect. \<close>
+  variables. Thus we first prove laws for these cases. \<close>
   
 lemma usubst_lookup_id [usubst]: "\<langle>id\<rangle>\<^sub>s x = var x"
   by (transfer, simp)
@@ -843,35 +308,20 @@ lemma usubst_upd_pr_var_id [usubst]:
   apply (auto)
   done
   
-lemma usubst_upd_comm_dash [usubst]:
-  fixes x :: "('a \<Longrightarrow> '\<alpha>)"
-  shows "\<sigma>($x\<acute> \<mapsto>\<^sub>s v, $x \<mapsto>\<^sub>s u) = \<sigma>($x \<mapsto>\<^sub>s u, $x\<acute> \<mapsto>\<^sub>s v)"
-  using out_in_indep usubst_upd_comm by blast
+
 
 lemma subst_upd_lens_plus [usubst]: 
   "subst_upd \<sigma> (x +\<^sub>L y) \<guillemotleft>(u,v)\<guillemotright> = \<sigma>(y \<mapsto>\<^sub>s \<guillemotleft>v\<guillemotright>, x \<mapsto>\<^sub>s \<guillemotleft>u\<guillemotright>)"
   by (simp add: lens_defs uexpr_defs subst_upd_uvar_def, transfer, auto)
 
-lemma subst_upd_in_lens_plus [usubst]: 
-  "subst_upd \<sigma> (ivar (x +\<^sub>L y)) \<guillemotleft>(u,v)\<guillemotright> = \<sigma>($y \<mapsto>\<^sub>s \<guillemotleft>v\<guillemotright>, $x \<mapsto>\<^sub>s \<guillemotleft>u\<guillemotright>)"
-  by (simp add: lens_defs uexpr_defs subst_upd_uvar_def, transfer, auto simp add: prod.case_eq_if)
 
-lemma subst_upd_out_lens_plus [usubst]: 
-  "subst_upd \<sigma> (ovar (x +\<^sub>L y)) \<guillemotleft>(u,v)\<guillemotright> = \<sigma>($y\<acute> \<mapsto>\<^sub>s \<guillemotleft>v\<guillemotright>, $x\<acute> \<mapsto>\<^sub>s \<guillemotleft>u\<guillemotright>)"
-  by (simp add: lens_defs uexpr_defs subst_upd_uvar_def, transfer, auto simp add: prod.case_eq_if)
     
 lemma usubst_lookup_upd_indep [usubst]:
   assumes "mwb_lens x" "x \<bowtie> y"
   shows "\<langle>\<sigma>(y \<mapsto>\<^sub>s v)\<rangle>\<^sub>s x = \<langle>\<sigma>\<rangle>\<^sub>s x"
   using assms
   by (simp add: subst_upd_uvar_def, transfer, simp)
-    
-text \<open> If a variable is unrestricted in a substitution then it's application has no effect. \<close>
-
-lemma usubst_apply_unrest [usubst]:
-  "\<lbrakk> vwb_lens x; x \<sharp> \<sigma> \<rbrakk> \<Longrightarrow> \<langle>\<sigma>\<rangle>\<^sub>s x = var x"
-  by (simp add: unrest_usubst_def, transfer, auto simp add: fun_eq_iff, metis vwb_lens_wb wb_lens.get_put wb_lens_weak weak_lens.put_get)
-
+   
 text \<open> There follows various laws about deleting variables from a substitution. \<close>
     
 lemma subst_del_id [usubst]:
@@ -886,223 +336,6 @@ lemma subst_del_upd_diff [usubst]:
   "x \<bowtie> y \<Longrightarrow> \<sigma>(y \<mapsto>\<^sub>s v) -\<^sub>s x = (\<sigma> -\<^sub>s x)(y \<mapsto>\<^sub>s v)"
   by (simp add: subst_del_def subst_upd_uvar_def lens_indep_comm)
 
-text \<open> If a variable is unrestricted in an expression, then any substitution of that variable
-  has no effect on the expression .\<close>
-    
-lemma subst_unrest [usubst]: "x \<sharp> P \<Longrightarrow> \<sigma>(x \<mapsto>\<^sub>s v) \<dagger> P = \<sigma> \<dagger> P"
-  by (simp add: subst_upd_uvar_def, transfer, auto)
-
-lemma subst_unrest_2 [usubst]: 
-  fixes P :: "('a, '\<alpha>) uexpr"
-  assumes "x \<sharp> P" "x \<bowtie> y"
-  shows "\<sigma>(x \<mapsto>\<^sub>s u,y \<mapsto>\<^sub>s v) \<dagger> P = \<sigma>(y \<mapsto>\<^sub>s v) \<dagger> P"
-  using assms
-  by (simp add: subst_upd_uvar_def, transfer, auto, metis lens_indep.lens_put_comm)
-
-lemma subst_unrest_3 [usubst]: 
-  fixes P :: "('a, '\<alpha>) uexpr"
-  assumes "x \<sharp> P" "x \<bowtie> y" "x \<bowtie> z"
-  shows "\<sigma>(x \<mapsto>\<^sub>s u, y \<mapsto>\<^sub>s v, z \<mapsto>\<^sub>s w) \<dagger> P = \<sigma>(y \<mapsto>\<^sub>s v, z \<mapsto>\<^sub>s w) \<dagger> P"
-  using assms
-  by (simp add: subst_upd_uvar_def, transfer, auto, metis (no_types, hide_lams) lens_indep_comm)
-
-lemma subst_unrest_4 [usubst]: 
-  fixes P :: "('a, '\<alpha>) uexpr"
-  assumes "x \<sharp> P" "x \<bowtie> y" "x \<bowtie> z" "x \<bowtie> u"
-  shows "\<sigma>(x \<mapsto>\<^sub>s e, y \<mapsto>\<^sub>s f, z \<mapsto>\<^sub>s g, u \<mapsto>\<^sub>s h) \<dagger> P = \<sigma>(y \<mapsto>\<^sub>s f, z \<mapsto>\<^sub>s g, u \<mapsto>\<^sub>s h) \<dagger> P"
-  using assms
-  by (simp add: subst_upd_uvar_def, transfer, auto, metis (no_types, hide_lams) lens_indep_comm)
-
-lemma subst_unrest_5 [usubst]: 
-  fixes P :: "('a, '\<alpha>) uexpr"
-  assumes "x \<sharp> P" "x \<bowtie> y" "x \<bowtie> z" "x \<bowtie> u" "x \<bowtie> v"
-  shows "\<sigma>(x \<mapsto>\<^sub>s e, y \<mapsto>\<^sub>s f, z \<mapsto>\<^sub>s g, u \<mapsto>\<^sub>s h, v \<mapsto>\<^sub>s i) \<dagger> P = \<sigma>(y \<mapsto>\<^sub>s f, z \<mapsto>\<^sub>s g, u \<mapsto>\<^sub>s h, v \<mapsto>\<^sub>s i) \<dagger> P"
-  using assms
-  by (simp add: subst_upd_uvar_def, transfer, auto, metis (no_types, hide_lams) lens_indep_comm)
-
-lemma subst_compose_upd [usubst]: "x \<sharp> \<sigma> \<Longrightarrow> \<sigma> \<circ> \<rho>(x \<mapsto>\<^sub>s v) = (\<sigma> \<circ> \<rho>)(x \<mapsto>\<^sub>s v) "
-  by (simp add: subst_upd_uvar_def, transfer, auto simp add: unrest_usubst_def)
-
-
-subsection \<open> Substitution laws \<close>
-  
-text \<open> We now prove the key laws that show how a substitution should be performed for every 
-  expression operator, including the core function operators, literals, variables, and the 
-  arithmetic operators. They are all added to the \emph{usubst} theorem attribute so that
-  we can apply them using the substitution tactic. \<close>
-    
-lemma id_subst [usubst]: "id \<dagger> v = v"
-  by (transfer, simp)
-
-lemma subst_lit [usubst]: "\<sigma> \<dagger> \<guillemotleft>v\<guillemotright> = \<guillemotleft>v\<guillemotright>"
-  by (transfer, simp)
-
-lemma subst_var [usubst]: "\<sigma> \<dagger> var x = \<langle>\<sigma>\<rangle>\<^sub>s x"
-  by (transfer, simp)
-
-lemma usubst_ulambda [usubst]: "\<sigma> \<dagger> (\<lambda> x \<bullet> P(x)) = (\<lambda> x \<bullet> \<sigma> \<dagger> P(x))"
-  by (transfer, simp)
-
-lemma unrest_usubst_del [unrest]: "\<lbrakk> vwb_lens x; x \<sharp> (\<langle>\<sigma>\<rangle>\<^sub>s x); x \<sharp> \<sigma> -\<^sub>s x \<rbrakk> \<Longrightarrow>  x \<sharp> (\<sigma> \<dagger> P)"
-  by (simp add: subst_del_def subst_upd_uvar_def unrest_uexpr_def unrest_usubst_def subst.rep_eq usubst_lookup.rep_eq)
-     (metis vwb_lens.put_eq)
-
-text \<open> We add the symmetric definition of input and output variables to substitution laws
-        so that the variables are correctly normalised after substitution. \<close>
-
-lemma subst_uop [usubst]: "\<sigma> \<dagger> uop f v = uop f (\<sigma> \<dagger> v)"
-  by (transfer, simp)
-
-lemma subst_bop [usubst]: "\<sigma> \<dagger> bop f u v = bop f (\<sigma> \<dagger> u) (\<sigma> \<dagger> v)"
-  by (transfer, simp)
-
-lemma subst_trop [usubst]: "\<sigma> \<dagger> trop f u v w = trop f (\<sigma> \<dagger> u) (\<sigma> \<dagger> v) (\<sigma> \<dagger> w)"
-  by (transfer, simp)
-
-lemma subst_case_prod [usubst]:
-  fixes P :: "'i \<Rightarrow> 'j \<Rightarrow> ('a, '\<alpha>) uexpr"  
-  shows "\<sigma> \<dagger> case_prod (\<lambda> x y. P x y) v = case_prod (\<lambda> x y. \<sigma> \<dagger> P x y) v"
-  by (simp add: case_prod_beta')
-
-lemma subst_plus [usubst]: "\<sigma> \<dagger> (x + y) = \<sigma> \<dagger> x + \<sigma> \<dagger> y"
-  by (simp add: plus_uexpr_def subst_bop)
-
-lemma subst_times [usubst]: "\<sigma> \<dagger> (x * y) = \<sigma> \<dagger> x * \<sigma> \<dagger> y"
-  by (simp add: times_uexpr_def subst_bop)
-
-lemma subst_mod [usubst]: "\<sigma> \<dagger> (x mod y) = \<sigma> \<dagger> x mod \<sigma> \<dagger> y"
-  by (simp add: mod_uexpr_def usubst)
-
-lemma subst_div [usubst]: "\<sigma> \<dagger> (x div y) = \<sigma> \<dagger> x div \<sigma> \<dagger> y"
-  by (simp add: divide_uexpr_def usubst)
-
-lemma subst_minus [usubst]: "\<sigma> \<dagger> (x - y) = \<sigma> \<dagger> x - \<sigma> \<dagger> y"
-  by (simp add: minus_uexpr_def subst_bop)
-
-lemma subst_uminus [usubst]: "\<sigma> \<dagger> (- x) = - (\<sigma> \<dagger> x)"
-  by (simp add: uminus_uexpr_def subst_uop)
-
-lemma subst_zero [usubst]: "\<sigma> \<dagger> 0 = 0"
-  by (simp add: zero_uexpr_def subst_lit)
-
-lemma subst_one [usubst]: "\<sigma> \<dagger> 1 = 1"
-  by (simp add: one_uexpr_def subst_lit)
-
-lemma subst_eq_upred [usubst]: "\<sigma> \<dagger> (x =\<^sub>u y) = (\<sigma> \<dagger> x =\<^sub>u \<sigma> \<dagger> y)"
-  by (simp add: eq_upred_def usubst)
-
-text \<open> This laws shows the effect of applying one substitution after another -- we simply
-  use function composition to compose them. \<close>
-    
-lemma subst_subst [usubst]: "\<sigma> \<dagger> \<rho> \<dagger> e = (\<rho> \<circ> \<sigma>) \<dagger> e"
-  by (transfer, simp)
-
-text \<open> The next law is similar, but shows how such a substitution is to be applied to every
-  updated variable additionally. \<close>
-    
-lemma subst_upd_comp [usubst]:
-  fixes x :: "('a \<Longrightarrow> '\<alpha>)"
-  shows "\<rho>(x \<mapsto>\<^sub>s v) \<circ> \<sigma> = (\<rho> \<circ> \<sigma>)(x \<mapsto>\<^sub>s \<sigma> \<dagger> v)"
-  by (rule ext, simp add:uexpr_defs subst_upd_uvar_def, transfer, simp)
-
-lemma subst_singleton:
-  fixes x :: "('a \<Longrightarrow> '\<alpha>)"
-  assumes "x \<sharp> \<sigma>"
-  shows "\<sigma>(x \<mapsto>\<^sub>s v) \<dagger> P = (\<sigma> \<dagger> P)\<lbrakk>v/x\<rbrakk>"
-  using assms
-  by (simp add: usubst)
-
-lemmas subst_to_singleton = subst_singleton id_subst
-
-subsection \<open> Ordering substitutions \<close>
-
-text \<open> A simplification procedure to reorder substitutions maplets lexicographically by variable syntax \<close>
-
-simproc_setup subst_order ("subst_upd_uvar (subst_upd_uvar \<sigma> x u) y v") =
-  {* (fn _ => fn ctx => fn ct => 
-        case (Thm.term_of ct) of
-          Const ("utp_subst.subst_upd_uvar", _) $ (Const ("utp_subst.subst_upd_uvar", _) $ s $ x $ u) $ y $ v
-            => if (YXML.content_of (Syntax.string_of_term ctx x) > YXML.content_of(Syntax.string_of_term ctx y))
-               then SOME (mk_meta_eq @{thm usubst_upd_comm})
-               else NONE  |
-          _ => NONE) 
-  *}
-
-subsection \<open> Unrestriction laws \<close>
-
-text \<open> These are the key unrestriction theorems for substitutions and expressions involving substitutions. \<close>
-  
-lemma unrest_usubst_single [unrest]:
-  "\<lbrakk> mwb_lens x; x \<sharp> v \<rbrakk> \<Longrightarrow> x \<sharp> P\<lbrakk>v/x\<rbrakk>"
-  by (transfer, auto simp add: subst_upd_uvar_def unrest_uexpr_def)
-
-lemma unrest_usubst_id [unrest]:
-  "mwb_lens x \<Longrightarrow> x \<sharp> id"
-  by (simp add: unrest_usubst_def)
-
-lemma unrest_usubst_upd [unrest]:
-  "\<lbrakk> x \<bowtie> y; x \<sharp> \<sigma>; x \<sharp> v \<rbrakk> \<Longrightarrow> x \<sharp> \<sigma>(y \<mapsto>\<^sub>s v)"
-  by (simp add: subst_upd_uvar_def unrest_usubst_def unrest_uexpr.rep_eq lens_indep_comm)
-
-lemma unrest_subst [unrest]:
-  "\<lbrakk> x \<sharp> P; x \<sharp> \<sigma> \<rbrakk> \<Longrightarrow> x \<sharp> (\<sigma> \<dagger> P)"
-  by (transfer, simp add: unrest_usubst_def)
-    
-subsection \<open> Conditional Substitution Laws \<close>
-  
-lemma usubst_cond_upd_1 [usubst]:
-  "\<sigma>(x \<mapsto>\<^sub>s u) \<triangleleft> b \<triangleright>\<^sub>s \<rho>(x \<mapsto>\<^sub>s v) = (\<sigma> \<triangleleft> b \<triangleright>\<^sub>s \<rho>)(x \<mapsto>\<^sub>s u \<triangleleft> b \<triangleright> v)"
-  by (simp add: cond_subst_def subst_upd_uvar_def uexpr_defs, transfer, auto)
-
-lemma usubst_cond_upd_2 [usubst]:
-  "\<lbrakk> vwb_lens x; x \<sharp> \<rho> \<rbrakk> \<Longrightarrow> \<sigma>(x \<mapsto>\<^sub>s u) \<triangleleft> b \<triangleright>\<^sub>s \<rho> = (\<sigma> \<triangleleft> b \<triangleright>\<^sub>s \<rho>)(x \<mapsto>\<^sub>s u \<triangleleft> b \<triangleright> &x)"
-  by (simp add: cond_subst_def subst_upd_uvar_def unrest_usubst_def uexpr_defs, transfer)
-     (metis (full_types, hide_lams) id_apply pr_var_def subst_upd_uvar_def usubst_upd_pr_var_id var.rep_eq)
- 
-lemma usubst_cond_upd_3 [usubst]:
-  "\<lbrakk> vwb_lens x; x \<sharp> \<sigma> \<rbrakk> \<Longrightarrow> \<sigma> \<triangleleft> b \<triangleright>\<^sub>s \<rho>(x \<mapsto>\<^sub>s v) = (\<sigma> \<triangleleft> b \<triangleright>\<^sub>s \<rho>)(x \<mapsto>\<^sub>s &x \<triangleleft> b \<triangleright> v)"
-  by (simp add: cond_subst_def subst_upd_uvar_def unrest_usubst_def uexpr_defs, transfer)
-     (metis (full_types, hide_lams) id_apply pr_var_def subst_upd_uvar_def usubst_upd_pr_var_id var.rep_eq)
-    
-lemma usubst_cond_id [usubst]:
-  "id \<triangleleft> b \<triangleright>\<^sub>s id = id"
-  by (auto simp add: cond_subst_def)
-    
-subsection \<open> Parallel Substitution Laws \<close>
-    
-lemma par_subst_id [usubst]:
-  "\<lbrakk> vwb_lens A; vwb_lens B \<rbrakk> \<Longrightarrow> id [A|B]\<^sub>s id = id"
-  by (simp add: par_subst_def id_def)
-
-lemma par_subst_left_empty [usubst]:
-  "\<lbrakk> vwb_lens A \<rbrakk> \<Longrightarrow> \<sigma> [\<emptyset>|A]\<^sub>s \<rho> = id [\<emptyset>|A]\<^sub>s \<rho>"
-  by (simp add: par_subst_def pr_var_def)
-
-lemma par_subst_right_empty [usubst]:
-  "\<lbrakk> vwb_lens A \<rbrakk> \<Longrightarrow> \<sigma> [A|\<emptyset>]\<^sub>s \<rho> = \<sigma> [A|\<emptyset>]\<^sub>s id"
-  by (simp add: par_subst_def pr_var_def)
-    
-lemma par_subst_comm:
-  "\<lbrakk> A \<bowtie> B \<rbrakk> \<Longrightarrow> \<sigma> [A|B]\<^sub>s \<rho> = \<rho> [B|A]\<^sub>s \<sigma>"
-  by (simp add: par_subst_def lens_override_def lens_indep_comm)
-      
-lemma par_subst_upd_left_in [usubst]:
-  "\<lbrakk> vwb_lens A; A \<bowtie> B; x \<subseteq>\<^sub>L A \<rbrakk> \<Longrightarrow> \<sigma>(x \<mapsto>\<^sub>s v) [A|B]\<^sub>s \<rho> = (\<sigma> [A|B]\<^sub>s \<rho>)(x \<mapsto>\<^sub>s v)"
-  by (simp add: par_subst_def subst_upd_uvar_def lens_override_put_right_in)
-     (simp add: lens_indep_comm lens_override_def sublens_pres_indep)
-
-lemma par_subst_upd_left_out [usubst]:
-  "\<lbrakk> vwb_lens A; x \<bowtie> A \<rbrakk> \<Longrightarrow> \<sigma>(x \<mapsto>\<^sub>s v) [A|B]\<^sub>s \<rho> = (\<sigma> [A|B]\<^sub>s \<rho>)"
-  by (simp add: par_subst_def subst_upd_uvar_def lens_override_put_right_out)
-     
-lemma par_subst_upd_right_in [usubst]:
-  "\<lbrakk> vwb_lens B; A \<bowtie> B; x \<subseteq>\<^sub>L B \<rbrakk> \<Longrightarrow> \<sigma> [A|B]\<^sub>s \<rho>(x \<mapsto>\<^sub>s v) = (\<sigma> [A|B]\<^sub>s \<rho>)(x \<mapsto>\<^sub>s v)"
-  using lens_indep_sym par_subst_comm par_subst_upd_left_in by fastforce
-
-lemma par_subst_upd_right_out [usubst]:
-  "\<lbrakk> vwb_lens B; A \<bowtie> B; x \<bowtie> B \<rbrakk> \<Longrightarrow> \<sigma> [A|B]\<^sub>s \<rho>(x \<mapsto>\<^sub>s v) = (\<sigma> [A|B]\<^sub>s \<rho>)"
-  by (simp add: par_subst_comm par_subst_upd_left_out)
-    
 
 
 
@@ -1114,35 +347,17 @@ lemma par_subst_upd_right_out [usubst]:
 
 
 
-named_theorems alpha
-
-method alpha_tac = (simp add: alpha unrest)?
-
-lift_definition aext :: "('a, '\<beta>) uexpr \<Rightarrow> ('\<beta>, '\<alpha>) lens \<Rightarrow> ('a, '\<alpha>) uexpr" (infixr "\<oplus>\<^sub>p" 95)
-is "\<lambda> P x b. P (get\<^bsub>x\<^esub> b)" .
-
-subsection \<open> Substitution Alphabet Extension \<close>
-
-text \<open> This allows us to extend the alphabet of a substitution, in a similar way to expressions. \<close>
-  
-definition subst_ext :: "'\<alpha> usubst \<Rightarrow> ('\<alpha> \<Longrightarrow> '\<beta>) \<Rightarrow> '\<beta> usubst" (infix "\<oplus>\<^sub>s" 65) where "\<sigma> \<oplus>\<^sub>s x = (\<lambda> s. put\<^bsub>x\<^esub> s (\<sigma> (get\<^bsub>x\<^esub> s)))"
-
-lemma id_subst_ext [usubst]:
-  "wb_lens x \<Longrightarrow> id \<oplus>\<^sub>s x = id"
-  by (metis eq_id_iff id_apply iso_tuple_surjective_proof_assist_def subst_ext_def wb_lens.source_stability wb_lens_def weak_lens.put_get weak_lens.update_def)
 
 
-    
-subsection \<open> Substitution Alphabet Restriction \<close>
 
-text \<open> This allows us to reduce the alphabet of a substitution, in a similar way to expressions. \<close>
-  
-definition subst_res :: "'\<alpha> usubst \<Rightarrow> ('\<beta> \<Longrightarrow> '\<alpha>) \<Rightarrow> '\<beta> usubst" (infix "\<restriction>\<^sub>s" 65) where
- "\<sigma> \<restriction>\<^sub>s x = (\<lambda> s. get\<^bsub>x\<^esub> (\<sigma> (create\<^bsub>x\<^esub> s)))"
 
-lemma id_subst_res [usubst]:
-  "mwb_lens x \<Longrightarrow> id \<restriction>\<^sub>s x = id"
-  by (metis eq_id_iff mwb_lens_weak subst_res_def weak_lens.create_get)
+
+
+
+
+
+
+
 
 
 
