nmap_test.thy
@@ -1,0 +1,26 @@
+
+theory nmap_test
+imports
+  nmap_assign
+begin
+
+
+alphabet state =
+  a :: int
+  b :: int 
+  c :: int
+
+theorem "(a,b) := (2+3, &b) = (a := 5)"
+  by (simp add:  usubst_upd_comm usubst_upd_var_id)
+
+theorem "(a,b,c) := (2, &b, 4) = (a,c) := (2,4)"
+  by (metis b_vwb_lens pr_var_def state_indeps(1) usubst_upd_comm usubst_upd_pr_var_id)
+
+theorem  "(a:=5) \<triangleleft> True \<triangleright>\<^sub>\<p> (b:=6) = (a:=5)"
+  by (simp add: ifprog_def)
+
+theorem (in nchoice) "(a:=3)  \<sqinter> (b:=4) =  (a:=4)  \<sqinter>  (b:=3)" 
+  by (simp add: nch_commute)
+
+
+end
